rocq-skylabs-brick/tests/member_pointer_encoding.v
@@ -1,0 +1,26 @@
+(*
+ * Copyright (c) 2026 SkyLabs AI, Inc.
+ * This software is distributed under the terms of the BedRock Open-Source License.
+ * See the LICENSE-BedRock file in the repository root for details.
+ *)
+Require Import skylabs.prelude.base.
+Require Import skylabs.lang.cpp.syntax.
+Require Import skylabs.lang.cpp.semantics.genv.
+Require Import skylabs.lang.cpp.semantics.types.
+Require Import skylabs.lang.cpp.model.simple_pred.
+
+Import SimpleCPP.
+
+Section with_genv.
+  Context `{Σ : cpp_logic} {σ : genv}.
+
+  Example member_pointer_encoding_matches_size cls ty v vs :
+    pure_encodes (Tmember_pointer cls ty) v vs ->
+    size_of σ (Tmember_pointer cls ty) = Some (N.of_nat (length vs)).
+  Proof. move=> /length_encodes ->. reflexivity. Qed.
+
+  Example undefined_member_pointer_encoding cls ty :
+    pure_encodes (Tmember_pointer cls ty) VALUES_DEFS_IMPL.Vundef
+      (repeat Rundef (bitsize.bytesNat (member_pointer_bitsize σ))).
+  Proof. reflexivity. Qed.
+End with_genv.
