rocq-skylabs-brick/tests/member_pointer_layout.v
@@ -1,0 +1,43 @@
+(*
+ * Copyright (c) 2026 SkyLabs AI, Inc.
+ * This software is distributed under the terms of the BedRock Open-Source License.
+ * See the LICENSE-BedRock file in the repository root for details.
+ *)
+Require Import skylabs.prelude.base.
+Require Import skylabs.lang.cpp.syntax.
+Require Import skylabs.lang.cpp.semantics.genv.
+Require Import skylabs.lang.cpp.semantics.types.
+
+#[local] Definition member_type : type := "int C::*"%cpp_type.
+
+#[local] Definition layout_env (sz : bitsize) : genv :=
+  {| genv_tu := empty_tu abi.x64_linux; member_pointer_bitsize := sz |}.
+
+(* The new parameter must not be replaced by the ordinary pointer width. *)
+Example distinct_pointer_widths :
+  pointer_size (layout_env bitsize.W128) = 8%N /\
+  size_of (layout_env bitsize.W128) member_type = Some 16%N.
+Proof. split; reflexivity. Qed.
+
+Example qualified_member_pointer_array :
+  size_of (layout_env bitsize.W32) (Tarray (Tconst member_type) 3) = Some 12%N.
+Proof. reflexivity. Qed.
+
+Example extension_cannot_change_member_pointer_width :
+  ~ genv_leq (layout_env bitsize.W64) (layout_env bitsize.W128).
+Proof. move=> /member_pointer_bitsize_le. discriminate. Qed.
+
+Section with_genv.
+  Context {σ : genv}.
+
+  Example member_pointer_size_instance cls ty :
+    SizeOf (Tmember_pointer cls ty) (member_pointer_size σ).
+  Proof. apply _. Qed.
+
+  Example member_pointer_alignment cls ty :
+    is_Some (@align_of σ (Tmember_pointer cls ty)).
+  Proof.
+    destruct (align_of_size_of' _ _ (size_of_member_pointer cls ty)) as [al [Hal _]].
+    by exists al.
+  Qed.
+End with_genv.
